$$
\begin{aligned}
V_{b1} &= V_{CC}·\frac{R_{b12}}{R_{b11}+R_{b12}}=3V \\
V_{e1} &= V_{b1}-0.7V = 2.3V \\
I_{c1} &= I_{e1} = \frac{V_e}{R_{e1}+R_{e2}} = 2.09mA \\
V_{c1} &= V_{CC} - I_{c1}R_{c1} = 7.82V \\
V_{ce1} &= V_{c1}-V_{e1} = 5.52V \\
\\
V_{b2} &= V_{CC}·\frac{R_{b22}}{R_{b21}+R_{b22}}=1.5V \\
V_{e2} &= V_{b2}-0.7V = 0.8V \\
I_{c2} &= I_{e2} = \frac{V_{e2}}{R_{e2}} = 0.73mA \\
V_{c2} &= V_{CC} - I_{c2}R_{c2} = 10.54V \\
V_{ce2} &= V_c-V_e = 9.74V
\end{aligned}
$$

$$
\begin{aligned}
A_{V1} &= \frac{V_{o}}{V_{i}} = \frac{-\beta R_{c}}{r_{be}+(1+\beta)R_{e}} \\
R_{i1} = 
\end{aligned}
$$

